Exceptions file completed (add List formalization) TODO: modif Ext_strutcture (FV_s... lemmas and others) with Lc proofs

2016/Exceptions.thy
@@ -7,34 +7,51 @@ begin
 
 datatype ltype=
 Unit | Fun ltype ltype (infixr "\<rightarrow>"  225) | VariantType "string list" "ltype list"("<(_):=(_)>" [201,200]225) |
-Ty string  
+Ty string | ListT ltype ("\<lambda>List (_)" 225) | Bool
 
 datatype lterm=
-  LVar nat 
+  LTrue
+| LFalse
+| LVar nat 
 | LApp lterm lterm 
 | LAbs ltype lterm 
 | unit
 | error
+| Lnil ltype 
+| Lcons ltype lterm lterm 
+| Lisnil ltype lterm 
+| Lhead ltype lterm 
+| Ltail ltype lterm
 
 
 fun shift_L :: "int \<Rightarrow> nat \<Rightarrow> lterm \<Rightarrow> lterm" where
  "shift_L d c (LVar k)    = LVar (if k < c then k else nat (int k + d))" |
  "shift_L d c (LApp t t1) = LApp (shift_L d c t) (shift_L d c t1)" |
  "shift_L d c (LAbs T t)  = LAbs T (shift_L d (Suc c) t)" |
- "shift_L d c error = error" |
- "shift_L d c unit = unit" 
+  "shift_L d c (Lisnil A t) = Lisnil A (shift_L d c t)"|
+  "shift_L d c (Lcons A t t') = Lcons A (shift_L d c t) (shift_L d c t')"|
+  "shift_L d c (Lhead A t) = Lhead A (shift_L d c t)"|
+  "shift_L d c (Ltail A t) = Ltail A (shift_L d c t)" |
+  "shift_L d c t = t"
 
 
 fun subst_L :: "nat \<Rightarrow> lterm \<Rightarrow> lterm \<Rightarrow> lterm" where
  "subst_L j s (LApp t1 t2) = LApp (subst_L j s t1) (subst_L j s t2)" |
  "subst_L j s (LVar k) = (if k = j then s else LVar k)" |
  "subst_L j s (LAbs T t) = LAbs T (subst_L (Suc j) (shift_L 1 0 s) t)"|
- "subst_L j s unit = unit" |
- "subst_L j s (error) = error"
+  "subst_L j s (Lisnil A t) = Lisnil A (subst_L j s t)"|
+  "subst_L j s (Lcons A t t') = Lcons A (subst_L j s t) (subst_L j s t')"|
+  "subst_L j s (Lhead A t) = Lhead A (subst_L j s t)" |
+  "subst_L j s (Ltail A t) = Ltail A (subst_L j s t)"|
+  "subst_L j s t = t"
 
 inductive is_value_L :: "lterm \<Rightarrow> bool" where
+  "is_value_L LTrue"|
+  "is_value_L LFalse"|
   "is_value_L unit"|
-  "is_value_L (LAbs T t)"
+  "is_value_L (LAbs T t)"|
+  VNil  :"is_value_L (Lnil A)"|
+  VCons :"is_value_L v1 \<Longrightarrow> is_value_L v2 \<Longrightarrow> is_value_L (Lcons A v1 v2)"
 
 
 inductive eval1_L :: "lterm \<Rightarrow> lterm \<Rightarrow> bool" where
@@ -49,7 +66,39 @@ inductive eval1_L :: "lterm \<Rightarrow> lterm \<Rightarrow> bool" where
   eval1_LErrApp1:
     "eval1_L (LApp error t) error"|
   eval1_LErrApp2:
-    "is_value_L v \<Longrightarrow> eval1_L (LApp v error) error" 
+    "is_value_L v \<Longrightarrow> eval1_L (LApp v error) error" |
+   eval1_Lcons1:
+    "eval1_L t t1 \<Longrightarrow> eval1_L (Lcons A t t') (Lcons A t1 t')"|
+  eval1_Lcons2:
+    "is_value_L v \<Longrightarrow> eval1_L t' t1 \<Longrightarrow> eval1_L (Lcons A v t') (Lcons A v t1)"|
+  eval1_LErrCons1:
+    "eval1_L (Lcons A error t) error"|
+  eval1_LErrCons2:
+    "is_value_L v \<Longrightarrow> eval1_L (Lcons A v error) error" |
+  eval1_Lisnil_nil:
+    "eval1_L (Lisnil A (Lnil A)) LTrue"|
+   eval1_Lisnil_cons:
+    "is_value_L v1 \<Longrightarrow> is_value_L v2 \<Longrightarrow> eval1_L (Lisnil A (Lcons A v1 v2)) LFalse"|
+  eval1_Lisnil_step:
+    "eval1_L t t' \<Longrightarrow> eval1_L (Lisnil A t) (Lisnil A t')"|
+  eval1_Lisnil_error:
+    "eval1_L (Lisnil A error) error"|
+  eval1_Lhead_cons:
+    "is_value_L v1 \<Longrightarrow> is_value_L v2 \<Longrightarrow> eval1_L (Lhead A (Lcons A v1 v2)) v1" | 
+  eval1_Lhead_step:
+    "eval1_L t t1 \<Longrightarrow> eval1_L (Lhead A t) (Lhead A t1)"|
+  eval1_Lhead_nil:
+    "eval1_L (Lhead A (Lnil B)) error"|
+  eval1_Lhead_error:
+    "eval1_L (Lhead A error) error" |
+  eval1_Ltail_cons:
+    "is_value_L v1 \<Longrightarrow> is_value_L v2 \<Longrightarrow> eval1_L (Ltail A (Lcons A v1 v2)) v2" | 
+  eval1_Ltail_step:
+    "eval1_L t t1 \<Longrightarrow> eval1_L (Ltail A t) (Ltail A t1)"|
+  eval1_Ltail_nil:
+    " eval1_L (Ltail A (Lnil B)) error"|
+  eval1_Ltail_error:
+    "eval1_L (Ltail A error) error"
  
   
 
@@ -64,6 +113,10 @@ abbreviation elem' :: "(nat \<times> ltype) \<Rightarrow> lcontext \<Rightarrow>
 
 
 inductive  has_type_L :: "lcontext \<Rightarrow> lterm \<Rightarrow> ltype \<Rightarrow> bool" ("((_)/ \<turnstile> (_)/ |:| (_))" [150, 150, 150] 150) where
+  has_type_LTrue:
+    "\<Gamma> \<turnstile> LTrue |:| Bool" |
+  has_type_LFalse:
+    "\<Gamma> \<turnstile> LFalse |:| Bool" |
   has_type_Lunit:
     "\<Gamma> \<turnstile> unit |:| Unit" |
   has_type_LVar:
@@ -73,24 +126,52 @@ inductive  has_type_L :: "lcontext \<Rightarrow> lterm \<Rightarrow> ltype \<Rig
   has_type_LApp:
     "\<Gamma> \<turnstile> t1 |:| (T11 \<rightarrow> T12) \<Longrightarrow> \<Gamma> \<turnstile> t2 |:| T11 \<Longrightarrow> \<Gamma> \<turnstile> (LApp t1 t2) |:| T12" |
   has_type_error:
-    "\<Gamma> \<turnstile> error |:| T"
-  
+    "\<Gamma> \<turnstile> error |:| T"|
+  has_type_Nil:
+    "\<Gamma> \<turnstile>  Lnil A  |:| \<lambda>List A"|
+  has_type_isNil:
+    "\<Gamma> \<turnstile>  t |:| \<lambda>List A \<Longrightarrow>\<Gamma> \<turnstile>  Lisnil A t |:| Bool"| 
+  has_type_head:
+    "\<Gamma> \<turnstile> t |:| \<lambda>List A \<Longrightarrow>\<Gamma> \<turnstile> Lhead A t |:| A"| 
+  has_type_tail:
+    "\<Gamma> \<turnstile> t |:| \<lambda>List A \<Longrightarrow>\<Gamma> \<turnstile> Ltail A t |:| \<lambda>List A"| 
+  has_type_cons:
+    "\<Gamma> \<turnstile> t |:| A \<Longrightarrow> \<Gamma> \<turnstile> t' |:| \<lambda>List A \<Longrightarrow>
+      \<Gamma> \<turnstile> Lcons A t t' |:| \<lambda>List A"  
+ 
+
+ 
 lemma canonical_forms:
+  "is_value_L v \<Longrightarrow> \<Gamma> \<turnstile> v |:| Bool \<Longrightarrow> v = LTrue \<or> v = LFalse"
   "is_value_L v \<Longrightarrow> \<Gamma> \<turnstile> v |:| Unit \<Longrightarrow> v = unit"
   "is_value_L v \<Longrightarrow> \<Gamma> \<turnstile> v |:| T1 \<rightarrow> T2 \<Longrightarrow> \<exists>t. v = LAbs T1 t"
-by (auto elim: has_type_L.cases is_value_L.cases)
+  "is_value_L v \<Longrightarrow> \<Gamma> \<turnstile> v |:| \<lambda>List A \<Longrightarrow> (\<exists>v1 v2. v = Lcons A v1 v2 \<and> is_value_L v1 \<and> is_value_L v2) \<or>
+                                          v = Lnil A"
+proof -
+  assume "is_value_L v" "\<Gamma> \<turnstile> v |:| \<lambda>List A"
+  then show "(\<exists>v1 v2. v = Lcons A v1 v2 \<and> is_value_L v1 \<and> is_value_L v2) \<or>
+                                          v = Lnil A"
+    by (induction rule:"is_value_L.induct") (auto elim: has_type_L.cases)
+qed (auto elim: has_type_L.cases is_value_L.cases)
 
 primrec FV :: "lterm \<Rightarrow> nat set" where
+ "FV LTrue = {}" |
+ "FV LFalse = {}" |
  "FV unit = {}" |
  "FV error = {}" |
  "FV (LVar x) = {x}" |
  "FV (LAbs T t) = image (\<lambda>x. x - 1) (FV t - {0})" |
- "FV (LApp t1 t2) = FV t1 \<union> FV t2" 
+ "FV (LApp t1 t2) = FV t1 \<union> FV t2"|
+  "FV (Lcons A t t') = FV t \<union> FV t'"|
+  "FV (Ltail A t) = FV t"|
+  "FV (Lhead A t) = FV t"|
+  "FV (Lisnil A t) = FV t"|
+  "FV (Lnil A) = {}" 
 
 definition is_closed :: "lterm \<Rightarrow> bool" where
   "is_closed t \<equiv> FV t = {}"
 
-(* 14.1.2 with try and raise structure*)
+
 theorem progress:
    "\<emptyset> \<turnstile> t |:| T \<Longrightarrow> is_closed t \<Longrightarrow> (\<forall>t'.\<not> eval1_L t t') \<Longrightarrow> is_value_L t \<or> t=error"
 proof (induction t T rule: has_type_L.induct)
@@ -98,7 +179,156 @@ proof (induction t T rule: has_type_L.induct)
     thus ?case 
       by (cases "is_value_L t1", cases "is_value_L t2")
           (auto intro: eval1_L.intros dest: canonical_forms simp: is_closed_def)
-qed (simp_all add: is_value_L.intros is_closed_def)
+next
+  case (has_type_isNil \<Gamma> t A)
+    note hyps=this
+    show ?case
+      using hyps(2,3,4) eval1_L.intros(10-13)
+            canonical_forms(4)[OF _ hyps(1)] is_closed_def
+      by (cases "\<exists>t'. eval1_L t t'")(blast, metis FV.simps(11))
+next
+  case (has_type_head \<Gamma> t A)
+    note hyps=this
+    show ?case
+      using hyps(2,3,4) eval1_L.intros(14-17)
+            canonical_forms(4)[OF _ hyps(1)] is_closed_def
+      by (cases "\<exists>t'. eval1_L t t'")(blast,metis FV.simps(10))
+next
+  case (has_type_tail \<Gamma> t A)
+    note hyps=this
+    show ?case
+      using hyps(2,3,4) eval1_L.intros(18-)
+            canonical_forms(4)[OF _ hyps(1)] is_closed_def
+      by (cases "\<exists>t'. eval1_L t t'")(blast,metis FV.simps(9))
+qed  (auto intro!: is_value_L.intros eval1_L.intros dest: canonical_forms simp: is_closed_def)+
+
+lemma simpl1: "nat (int x + 1) = Suc x" by simp
+lemma simpl2: "nat (1 + int x) = Suc x" by simp
+lemma simpl3: "nat (int x - 1) = x - 1" by simp
+
+lemma gr_Suc_conv: "Suc x \<le> n \<longleftrightarrow> (\<exists>m. n = Suc m \<and> x \<le> m)"
+  by (cases n) auto
+
+lemma FV_shift:
+  "FV (shift_L (int d) c t) = image (\<lambda>x. if x \<ge> c then x + d else x) (FV t)"
+proof (induction t arbitrary: c rule: lterm.induct)
+  case (LAbs T t)
+  thus ?case  by (auto simp: gr_Suc_conv image_iff) force+
+qed auto
+
+lemma FV_subst:
+  "FV (subst_L n t u) = (if n \<in> FV u then (FV u - {n}) \<union> FV t else FV u)"
+proof (induction u arbitrary: n t rule: lterm.induct)
+  case (LAbs T u)
+    have A: "Suc n \<in> FV u \<Longrightarrow> \<exists>x\<in>FV u - {0}. n = x - Suc 0 \<Longrightarrow>
+              {y. \<exists>x\<in>FV u - {Suc n} \<union> {y. \<exists>x\<in>FV t. y = Suc x} - {0}. y = x - Suc 0} =
+              {y. \<exists>x\<in>FV u - {0}. y = x - Suc 0} - {n} \<union> FV t"
+      by (rule, force) 
+          (rule, simp, metis (mono_tags, lifting) Diff_iff Un_iff diff_Suc_Suc 
+                              diff_zero mem_Collect_eq nat.simps(3) singletonD)      
+    have " Suc n \<in> FV u \<Longrightarrow>
+          \<forall>x\<in>FV u - {0}. n \<noteq> x - Suc 0 \<Longrightarrow>
+          {y. \<exists>x\<in>FV u - {Suc n} \<union> {y. \<exists>x\<in>FV t. y = Suc x} - {0}. y = x - Suc 0} =
+          {y. \<exists>x\<in>FV u - {0}. y = x - Suc 0}"
+      by (rule, rule ,simp , metis (mono_tags, lifting) Diff_iff diff_Suc_Suc diff_zero nat.simps(3) singletonD)+
+    
+    with A LAbs show ?case
+      by (auto simp:gr0_conv_Suc image_iff image_def FV_shift[of 1, unfolded int_1])      
+qed (auto simp: gr0_conv_Suc image_iff FV_shift[of 1, unfolded int_1])
+
+lemma weakening:
+  "\<Gamma> \<turnstile> t |:| T \<Longrightarrow> n \<le> length \<Gamma> \<Longrightarrow> insert_nth n U \<Gamma> \<turnstile> shift_L 1 n t |:| T"
+proof (induction \<Gamma> t T arbitrary: n rule: has_type_L.induct)
+  case (has_type_LAbs \<Gamma> T1 t T2)
+    from has_type_LAbs has_type_LAbs.hyps
+      has_type_LAbs.IH[where n="Suc n"] 
+    show ?case      
+      by (auto intro: has_type_L.intros)
+qed (auto simp: nth_append min_def simpl1 simpl2 simpl3 intro: has_type_L.intros)
+
+lemma substitution:
+  "\<Gamma> \<turnstile> t |:| T \<Longrightarrow> \<Gamma> \<turnstile> LVar n |:| U \<Longrightarrow> \<Gamma> \<turnstile> s |:| U \<Longrightarrow> 
+    \<Gamma> \<turnstile> subst_L n s t |:| T"  
+proof (induction \<Gamma> t T arbitrary: s n rule: has_type_L.induct)
+  case (has_type_LAbs \<Gamma> T1 t T2)
+    note hyps=this 
+   
+    show ?case
+      using hyps  has_type_L.simps[of _ "LVar _", simplified]
+            weakening[where n=0, simplified]
+      by (force intro!: "has_type_L.has_type_LAbs") 
+qed (auto intro!: has_type_L.intros simp: has_type_L.simps[of _ "LVar _" _, simplified])
+
+
+lemma shift_down:
+  "insert_nth n U \<Gamma> \<turnstile> t |:| T \<Longrightarrow> n \<le> length \<Gamma> \<Longrightarrow>
+   (\<And>x. x \<in> FV t \<Longrightarrow> x \<noteq> n) \<Longrightarrow> \<Gamma> \<turnstile> shift_L (- 1) n t |:| T"
+proof (induction "insert_nth n U \<Gamma>" t T arbitrary: \<Gamma> n rule: has_type_L.induct)
+  case (has_type_LAbs  V t T \<Gamma>)
+    note hyps=this
+    show ?case
+      using hyps hyps(2)[of "Suc n" "\<Gamma>|,|V"]
+      by (fastforce intro!: has_type_L.intros)     
+qed (fastforce intro: has_type_L.intros simp: nth_append min_def simpl1 simpl2 simpl3)+
+
+method inv_eval = (match premises in "eval1_L t t1" for t t1 \<Rightarrow>
+                    \<open> insert eval1_L.simps[of t t1] \<close>)
+
+lemma preservation:
+  "\<Gamma> \<turnstile> t |:| T\<Longrightarrow> eval1_L t t' \<Longrightarrow> \<Gamma> \<turnstile> t' |:| T"
+proof (induction arbitrary: t' rule: has_type_L.induct)
+  case (has_type_LApp \<Gamma> t1 T1 T2 t2)
+    note hyps=this
+    have "\<And>L TL T t12. t1 = LAbs T t12 \<Longrightarrow> t'=shift_L (-1) 0 (subst_L 0 (shift_L 1 0 t2) t12) \<Longrightarrow> ?case"
+      proof -
+        fix L TL T t12
+        assume t'_def:"t' = shift_L (- 1) 0 (subst_L 0 (shift_L 1 0 t2) t12)"
+               and Abs_t1: "t1 = LAbs T t12"
+        have t12_type:"\<Gamma> |,| T1 \<turnstile> t12 |:| T2"              
+          using hyps(1)[unfolded Abs_t1, simplified]
+                has_type_L.simps[of \<Gamma> "LAbs T  t12" "T1\<rightarrow>T2", simplified]
+          by blast+
+        have not_free0:"\<And>x. x \<in> FV (subst_L 0 (shift_L 1 0 t2) t12) \<Longrightarrow> x \<noteq> 0"
+          using FV_subst[of 0 "shift_L 1 0 t2" t12] 
+                FV_shift[of 1 0 t2, unfolded int_1]
+          by (cases "0\<in>FV t12") force+
+        from t'_def show ?case
+          using substitution[OF t12_type, of 0 T1 "shift_L 1 0 t2"] 
+                shift_down[of 0 T1 \<Gamma> _ T2, simplified, unfolded neq0_conv[symmetric]]
+                weakening[OF hyps(2),of 0 T1, simplified]
+                not_free0
+                "has_type_L.simps"[of "\<Gamma>|,|T1" "LVar 0" T1,simplified]
+          by blast
+      qed
+
+    then show ?case 
+      using hyps(1-4) hyps(5)[unfolded eval1_L.simps[of "LApp _ _", simplified]]
+            has_type_L.intros(4,6,7)
+      by blast                 
+next
+  case (has_type_head \<Gamma> t A t')
+    note hyps=this and inv=this(3)[unfolded eval1_L.simps[of "Lhead _ _", simplified]]
+    show ?case
+      using inv has_type_L.intros(10)[OF hyps(2)] hyps(1)
+            has_type_L.simps[of \<Gamma> "Lcons _ _ _" "\<lambda>List A", simplified]
+            has_type_error
+      by blast
+next
+  case (has_type_tail \<Gamma> t A t')
+    note hyps=this and inv=this(3)[unfolded eval1_L.simps[of "Ltail _ _", simplified]]
+    show ?case
+      using inv has_type_L.intros(11)[OF hyps(2)] hyps(1)
+            has_type_L.simps[of \<Gamma> "Lcons _ _ _" "\<lambda>List A", simplified]
+            has_type_error
+      by blast
+next
+  case (has_type_isNil \<Gamma> t A)
+     note hyps=this and inv=this(3)[unfolded eval1_L.simps[of "Lisnil _ _", simplified]]
+    show ?case
+      using inv has_type_L.intros(1,2) has_type_L.intros(9)[OF hyps(2)] hyps(1)
+            has_type_error
+      by meson
+qed (inv_eval, force intro!: has_type_L.intros)+
 
 
 datatype lterm1=
@@ -108,7 +338,6 @@ datatype lterm1=
 | unit1
 | trapp lterm1 lterm1 ("try/ (_)/ with/ (_)" [181,180]220)
 | raise lterm1
-| N nat
 | S string
 | Variant string lterm1 ltype ("<(_)::=(_)>/ as/ (_)" [201,200] 220)
 
@@ -141,20 +370,11 @@ primrec FV1 :: "lterm1 \<Rightarrow> nat set" where
  "FV1 (try t with t1) = FV1 t \<union> FV1 t1"|
  "FV1 (raise t) = FV1 t"|
  "FV1 (<s::=t> as A) = FV1 t"|
- "FV1 (N _) = {}"|
  "FV1 (S _) = {}"
-
-fun Errors:: "lterm1 \<Rightarrow> lterm1 set" where
- "Errors (LAbs1 T <L:=TL> t) = Errors t" |
- "Errors (LApp1 t1 t2) = Errors t1 \<union> Errors t2"|
- "Errors (try t with t1) = Errors t1"|
- "Errors (raise t) = {t}"|
- "Errors (<s::=t> as A) = Errors t"|
- "Errors _ = {}"
  
 
 inductive is_value_L1 :: "lterm1 \<Rightarrow> bool" where
-  "is_value_L1 unit1"|"is_value_L1 (N _)"|"is_value_L1 (S _)"|
+  "is_value_L1 unit1"|"is_value_L1 (S _)"|
   "is_value_L1 (LAbs1 T <L:=TL> t)" 
   |"is_value_L1 v \<Longrightarrow> is_value_L1 (<s::=v> as A)"
 
@@ -189,16 +409,11 @@ inductive eval1_L1 :: "lterm1 \<Rightarrow> lterm1 \<Rightarrow> bool" where
 inductive  has_type1_L :: "ltype \<Rightarrow> lcontext \<Rightarrow> lterm1 \<Rightarrow> ltype \<Rightarrow> bool" ("((_)|*|(_)/ \<turnstile>\<^sub>1 (_)/ |:| (_))" [150, 150, 150] 150) where
   has_type1_Lunit:
     "T\<alpha>|*|\<Gamma> \<turnstile>\<^sub>1 unit1 |:| Unit" |
-  has_type1_LNat:
-    "T\<alpha>|*|\<Gamma> \<turnstile>\<^sub>1 (N n) |:| Ty ''nat''"|
   has_type1_LString:
     "T\<alpha>|*|\<Gamma> \<turnstile>\<^sub>1 (S s) |:| Ty ''str''"|
   has_type1_LVar:
     "(x, T) |\<in>| \<Gamma> \<Longrightarrow> T\<alpha>|*|\<Gamma> \<turnstile>\<^sub>1 (LVar1 x) |:| T" |
-  has_type1_LAbs_empty:
-    "length L>0 \<Longrightarrow>distinct L \<Longrightarrow> length L = length TL \<Longrightarrow> <L:=TL>|*|(\<Gamma> |,| T1) \<turnstile>\<^sub>1 t2 |:| T2 \<Longrightarrow> 
-      <\<emptyset>:=\<emptyset>>|*|\<Gamma> \<turnstile>\<^sub>1 (LAbs1 T1 <L:=TL> t2) |:| (T1 \<rightarrow> T2)" |
-  has_type1_LAbs_sub:
+  has_type1_LAbs:
     " distinct L \<Longrightarrow> length L = length TL \<Longrightarrow> <L:=TL>|*|(\<Gamma> |,| T1) \<turnstile>\<^sub>1 t2 |:| T2 \<Longrightarrow> 
       <L:=TL>|*|\<Gamma> \<turnstile>\<^sub>1 (LAbs1 T1 <L:=TL> t2) |:| (T1 \<rightarrow> T2)" |
   has_type1_LApp:
@@ -212,6 +427,8 @@ inductive  has_type1_L :: "ltype \<Rightarrow> lcontext \<Rightarrow> lterm1 \<R
 
 method invert_type = (match premises in H:"Ta|*|\<Gamma> \<turnstile>\<^sub>1 Te |:| A" for Ta \<Gamma> Te A \<Rightarrow>
                         \<open> insert has_type1_L.simps[of Ta \<Gamma> Te A, simplified]\<close>)
+
+thm has_type1_L.induct
 
 lemma canonical_forms1:
   "is_value_L1 v \<Longrightarrow> T\<alpha>|*|\<Gamma> \<turnstile>\<^sub>1 v |:| Unit \<Longrightarrow> v = unit1"
@@ -236,23 +453,18 @@ next
   case (has_type1_Variant i L TL t)
     note hyps=this
     show ?case 
-      using hyps(3,4) "is_value_L1.intros"(5)[of t "L!i"]
+      using hyps(3,4) "is_value_L1.intros"(4)[of t "L!i"]
             eval1_VE[of t _ "L!i"] has_type1_L.simps[of "<\<emptyset>:=\<emptyset>>" \<emptyset> "raise _", simplified]
       by meson
 next
-  case (has_type1_try t T t2)
+  case (has_type1_try t1 T t2)
     note hyps=this
     show ?case
       using hyps(3) eval1_L1TryV eval1_L1TryE eval1_TryRaise
       by blast
 qed (simp_all add: is_value_L1.intros)
 
-lemma[simp]: "nat (int x + 1) = Suc x" by simp
-lemma[simp]: "nat (1 + int x) = Suc x" by simp
-lemma[simp]: "nat (int x - 1) = x - 1" by simp
 
-lemma gr_Suc_conv: "Suc x \<le> n \<longleftrightarrow> (\<exists>m. n = Suc m \<and> x \<le> m)"
-  by (cases n) auto
 
 lemma FV1_shift:
   "FV1 (shift_L1 (int d) c t) = image (\<lambda>x. if x \<ge> c then x + d else x) (FV1 t)"
@@ -279,75 +491,42 @@ proof (induction u arbitrary: n t rule: lterm1.induct)
     
     with A LAbs1 show ?case
       by (auto simp:gr0_conv_Suc image_iff image_def FV1_shift[of 1, unfolded int_1])      
-   
 qed (auto simp: gr0_conv_Suc image_iff FV1_shift[of 1, unfolded int_1])
 
 lemma weakening1:
   "T\<alpha>|*|\<Gamma> \<turnstile>\<^sub>1 t |:| T \<Longrightarrow> n \<le> length \<Gamma> \<Longrightarrow> T\<alpha>|*|insert_nth n U \<Gamma> \<turnstile>\<^sub>1 shift_L1 1 n t |:| T"
 proof (induction T\<alpha> \<Gamma> t T arbitrary: n rule: has_type1_L.induct)
-  case (has_type1_LAbs_empty L TL \<Gamma> t T1 T2)
-    from has_type1_LAbs_empty.prems has_type1_LAbs_empty.hyps(1-)
-      has_type1_LAbs_empty.IH[where n="Suc n"] 
+  case (has_type1_LAbs L TL \<Gamma> T1 t T2)
+    from has_type1_LAbs has_type1_LAbs.hyps
+      has_type1_LAbs.IH[where n="Suc n"] 
     show ?case      
       by (auto intro: has_type1_L.intros)
-next
-  case (has_type1_LAbs_sub L TL \<Gamma> T1 t T2)
-    from has_type1_LAbs_sub.prems has_type1_LAbs_sub.hyps
-      has_type1_LAbs_sub.IH[where n="Suc n"] 
-    show ?case      
-      by (auto intro: has_type1_L.intros)
-qed (auto simp: nth_append min_def intro: has_type1_L.intros)
+qed (auto simp: nth_append min_def simpl1 simpl2 simpl3 intro: has_type1_L.intros)
 
-
-
-lemma "<\<emptyset>:=\<emptyset>>|*|\<Gamma> \<turnstile>\<^sub>1 t |:| A \<Longrightarrow> Errors t ={}"
-proof (induction "<\<emptyset>:=\<emptyset>>::ltype" \<Gamma> t A rule: has_type1_L.induct)
-  case (has_type1_LAbs_empty L TL \<Gamma> T1 t T2)
-    thus ?case
-      sorry
-qed simp_all
-
-lemma substitution:
+lemma substitution1:
   "T\<alpha>|*|\<Gamma> \<turnstile>\<^sub>1 t |:| T \<Longrightarrow> T\<alpha>|*|\<Gamma> \<turnstile>\<^sub>1 LVar1 n |:| U \<Longrightarrow> T\<alpha>|*|\<Gamma> \<turnstile>\<^sub>1 s |:| U \<Longrightarrow> 
     T\<alpha>|*|\<Gamma> \<turnstile>\<^sub>1 subst_L1 n s t |:| T"  
 proof (induction T\<alpha> \<Gamma> t T arbitrary: s n rule: has_type1_L.induct)
-  case (has_type1_LAbs_empty L TL \<Gamma> T1 t T2)
-    note hyps=this
-    show ?case
-      apply simp
-      apply rule
-      using hyps(1-3)
-      apply force+
-      using hyps(4,5-) weakening1[where n=0 and U=T1]
-            has_type1_L.simps[of _ _ "LVar1 _", simplified] has_type1_LVar
-      sorry      
-next
-  case (has_type1_LAbs_sub L TL T\<alpha> \<Gamma> T1 t T2)
+  case (has_type1_LAbs L TL T\<alpha> \<Gamma> T1 t T2)
     note hyps=this 
    
     show ?case
       using hyps(1,2,4-)  has_type1_L.simps[of _ _ "LVar1 _", simplified]
             weakening1[where n=0, simplified]
-      by (force intro!: "has_type1_L.has_type1_LAbs_sub") 
+      by (force intro!: "has_type1_L.has_type1_LAbs") 
 qed (auto intro!: has_type1_L.intros simp: has_type1_L.simps[of _ _ "LVar1 _" _, simplified])
 
 
-lemma shift_down:
+lemma shift_down1:
   "T\<alpha>|*|(insert_nth n U \<Gamma>) \<turnstile>\<^sub>1 t |:| T \<Longrightarrow> n \<le> length \<Gamma> \<Longrightarrow>
    (\<And>x. x \<in> FV1 t \<Longrightarrow> x \<noteq> n) \<Longrightarrow> T\<alpha>|*|\<Gamma> \<turnstile>\<^sub>1 shift_L1 (- 1) n t |:| T"
 proof (induction T\<alpha> "insert_nth n U \<Gamma>" t T arbitrary: \<Gamma> n rule: has_type1_L.induct)
-  case (has_type1_LAbs_empty L TL V t T \<Gamma>)
-    note hyps=this
-    show ?case
-      using hyps(1-3,6-) hyps(5)[of "Suc n" "\<Gamma>|,|V"]
-      by (fastforce intro: has_type1_L.intros )
-next
-  case (has_type1_LAbs_sub L TL V t T \<Gamma>)
+  case (has_type1_LAbs L TL V t T \<Gamma>)
     note hyps=this
     show ?case
       using hyps(1,2,5-) hyps(4)[of "Suc n" "\<Gamma>|,|V"]
       by (fastforce intro: has_type1_L.intros )     
-qed (fastforce intro: has_type1_L.intros simp: nth_append min_def)+
+qed (fastforce intro: has_type1_L.intros simp: nth_append min_def simpl1 simpl2 simpl3)+
 
 
 method invert_eval1 = (match premises in H:"eval1_L1 Te Te1" (multi) for Te Te1::lterm1 \<Rightarrow>
@@ -359,7 +538,7 @@ method raise_solve = (match conclusion in "Ta|*|\<Gamma> \<turnstile>\<^sub>1 ra
                              \<close>\<close>, (fastforce intro:has_type1_L.intros))
 
 
-lemma preservation:
+lemma preservation1:
   " T\<alpha>|*|\<Gamma> \<turnstile>\<^sub>1 t |:| T\<Longrightarrow> eval1_L1 t t' \<Longrightarrow> T\<alpha>|*|\<Gamma> \<turnstile>\<^sub>1 t' |:| T"
 proof (induction arbitrary: t' rule: has_type1_L.induct)
   case (has_type1_try L TL \<Gamma> t1 T1 t2)
@@ -376,7 +555,7 @@ next
         assume t'_def:"t' = shift_L1 (- 1) 0 (subst_L1 0 (shift_L1 1 0 t2) t12)"
                and Abs_t1: "t1 = LAbs1 T <L:=TL> t12"
         have t12_type:"<L:=TL>|*|\<Gamma> |,| T1 \<turnstile>\<^sub>1 t12 |:| T2" and 
-              T\<alpha>_def : "T\<alpha> = <\<emptyset>:=\<emptyset>> \<or> T\<alpha> = <L:=TL>"
+              T\<alpha>_def : "T\<alpha> = <L:=TL>"
           using hyps(1)[unfolded Abs_t1, simplified]
                 has_type1_L.simps[of T\<alpha> \<Gamma> "LAbs1 T <L:=TL> t12" "T1\<rightarrow>T2", simplified]
           by blast+
@@ -385,20 +564,17 @@ next
                 FV1_shift[of 1 0 t2, unfolded int_1]
           by (cases "0\<in>FV1 t12") force+
         from t'_def show ?case
-          using T\<alpha>_def
-          apply auto
-          defer
-          using substitution[OF t12_type, of 0 T1 "shift_L1 1 0 t2"] 
-                shift_down[of _ 0 T1 \<Gamma> _ T2, simplified, unfolded neq0_conv[symmetric]]
+          using T\<alpha>_def substitution1[OF t12_type, of 0 T1 "shift_L1 1 0 t2"] 
+                shift_down1[of _ 0 T1 \<Gamma> _ T2, simplified, unfolded neq0_conv[symmetric]]
                 weakening1[OF hyps(2),of 0 T1, simplified]
                 not_free0
                 "has_type1_L.simps"[of "<L:=TL>" "\<Gamma>|,|T1" "LVar1 0" T1,simplified]
-          apply blast
-          
-          (*by blast  *) sorry
+          by blast
       qed
+
     with has_type1_LApp show ?case
       by simp (invert_eval1, (meson has_type1_L.intros;(raise_solve|blast)))
+
 qed (raise_solve|(invert_eval1, meson has_type1_L.intros), (raise_solve?))+
 
 
